high/Veritas.MultiSetHash.fst
@@ -1,0 +1,310 @@
+module Veritas.MultiSetHash
+
+open FStar.BitVector
+open FStar.Seq
+open Veritas.Key
+open Veritas.MultiSet
+open Veritas.Record
+open Veritas.SeqAux
+include Veritas.MultiSetHashDomain
+module T = Veritas.Formats.Types
+module VF = Veritas.Formats
+module U8 = FStar.UInt8
+module U64 = FStar.UInt64
+module L = FStar.List.Tot.Properties
+open Veritas.BinTree
+open FStar.Mul
+module BV = FStar.BV
+module HA = Veritas.Steel.HashAccumulator
+
+(* This module specifies a hash on a sequence of ms_hasfn_dom entries.
+
+   Concretely, it corresponds on part of its domain to the hash
+   function implemented in Veritas.Steel.PRFSetHash
+
+   However ms_hashfn_dom is a larger type than the domain of
+   Veritas.Steel.PRFSetHash. In particular, ms_hashfn_dom includes
+
+     - arbitrary integers in data values (whereas in the Steel code,
+       values are just u256)
+
+     - arbitrary natural numbers for timestamp and epoch counts
+       (whereas in Steel, each is only 32 bits)
+
+     - arbitrary natural numbers of thread ids (whereas in Steel they
+       are a u16)
+
+     So, for ms_hashfn_dom elements that do not meet these bounds, we
+     rely on unspecified_hash_function. Otherwise, we use what is
+     specified by PRFSetHash.
+
+     This "overspecification" of the hash on the full domain of
+     ms_hashfn_dom doesn't hurt us, since eventually, we will only
+     relate the low-level hashes computed on the sub-domain of values
+     of ms_hashfn_dom that are represented in Steel.
+
+*)
+assume
+val unspecified_hash_function (e: ms_hashfn_dom)
+  : Tot HA.hash_value_t
+
+(* A total serializer for stamped records
+   -- This assumption is a technicality.
+
+      The serializer spec produced by EverParse is in the GTot
+      effect. Whereas we want a Tot serializer here ... or else we
+      could move the entire high and intermediate development to
+      GTot. Which would be fine too but is a big syntactic change.
+
+      Instead, we assume a total serializer that is extensionally
+      equal to the EverParse serializer spec
+*)
+assume
+val serializer (e:T.stamped_record)
+  : Tot (s:seq UInt8.t{ s == VF.serialize_stamped_record_spec e })
+
+[@@"opaque_to_smt"]
+let lseq8_to_u8 (l:lseq bool 8)
+  : U8.t
+  = U8.uint_to_t (BV.bv2int (FStar.BV.list2bv (Seq.seq_to_list l)))
+
+[@@"opaque_to_smt"]
+let lseq64_to_u64 (s:lseq bool 64)
+  : U64.t
+  = U64.uint_to_t (BV.bv2int (BV.list2bv (seq_to_list s)))
+
+[@@"opaque_to_smt"]
+let lseq256_as_u256 (l:lseq bool 256)
+  : T.u256
+  = let v3, rest = Seq.split l 64 in
+    let v2, rest = Seq.split rest 64 in
+    let v1, v0 = Seq.split rest 64 in
+    {
+      v3 = lseq64_to_u64 v3;
+      v2 = lseq64_to_u64 v2;
+      v1 = lseq64_to_u64 v1;
+      v0 = lseq64_to_u64 v0
+    }
+
+[@@"opaque_to_smt"]
+let rec bv_to_lseq_u8 (#n:nat) (l:lseq bool (8 * n))
+  : lseq U8.t n
+  = if n = 0 then Seq.empty
+    else let h, rest = Seq.split l 8 in
+         Seq.cons (lseq8_to_u8 h) (bv_to_lseq_u8 #(n - 1) rest)
+
+[@@"opaque_to_smt"]
+let rec lseq_u8_to_bv (#n:nat) (l:lseq U8.t n)
+  : lseq bool (8 * n)
+  = if n = 0 then Seq.empty
+    else let hd = Seq.seq_of_list (BV.bv2list (BV.int2bv #8 (U8.v (Seq.head l)))) in
+         Seq.append hd (lseq_u8_to_bv #(n - 1) (Seq.tail l))
+
+[@@"opaque_to_smt"]
+let rec key_as_seq (k:key)
+  : lseq bool (depth k)
+  = match k with
+    | Root -> Seq.empty
+    | LeftChild k' -> Seq.snoc (key_as_seq k') false
+    | RightChild k' -> Seq.snoc (key_as_seq k') true
+
+[@@"opaque_to_smt"]
+let key_as_lseq_256 (k:key)
+  : lseq bool 256
+  = let s = key_as_seq k in
+    let pad = Seq.create (256 - depth k) false in
+    Seq.append pad s
+
+[@@"opaque_to_smt"]
+let key_as_u256 (k:key)
+  : Tot T.u256
+  = lseq256_as_u256 (key_as_lseq_256 k)
+
+let as_key (k:key)
+  : T.key
+  = { k = key_as_u256 k;
+      significant_digits = FStar.UInt16.uint_to_t (depth k) }
+
+let hash_value_as_hash_value (h:hash_value)
+  : T.hash_value
+  = lseq256_as_u256 h
+
+let desc_hash_as_descendent_hash (dh:desc_hash)
+  : T.descendent_hash
+  = match dh with
+    | Empty -> T.Dh_vnone ()
+    | Desc k v b ->
+      let k = as_key k in
+      let v = hash_value_as_hash_value v in
+      T.Dh_vsome T.({ dhd_key = k; dhd_h = v; evicted_to_blum = if b then Vtrue else Vfalse })
+
+let merkle_value_as_mval_value (mv:merkle_value)
+  : T.mval_value
+  = { l = desc_hash_as_descendent_hash mv.l;
+      r = desc_hash_as_descendent_hash mv.r }
+
+[@@"opaque_to_smt"]
+let data_value_as_data_value (mv:data_value)
+  : option T.data_value
+  = match mv with
+    | Null -> Some (T.Dv_vnone ())
+    | DValue i ->
+      if 0 <= i && i < pow2 256
+      then Some (T.Dv_vsome (lseq256_as_u256 (Seq.seq_of_list (BV.bv2list (BV.int2bv #256 i)))))
+      else None
+
+let as_value (v:value)
+  : option T.value
+  = match v with
+    | MVal mv ->
+      Some (T.V_mval (merkle_value_as_mval_value mv))
+    | DVal v ->
+      let vopt = data_value_as_data_value v in
+      match vopt with
+      | Some v -> Some (T.V_dval v)
+      | _ -> None
+
+let as_record (r:record)
+  : option T.record
+  = match as_value (snd r) with
+    | None -> None
+    | Some v ->
+      Some T.({ record_key = as_key (fst r);
+                record_value = v })
+
+let as_stamped_record (e:ms_hashfn_dom)
+  : option T.stamped_record
+  = let r = as_record e.r in
+    if Some? r
+    && e.t.e < pow2 32
+    && e.t.c < pow2 32
+    && e.i < pow2 16
+    then (
+      let t = U64.uint_to_t e.t.e in
+      let c = U64.uint_to_t e.t.c in
+      let i = FStar.UInt16.uint_to_t e.i in
+      let ts = U64.logxor (U64.shift_left t 32ul) c in
+      Some T.({
+             sr_record = Some?.v r;
+             sr_timestamp = ts;
+             sr_thread_id = i
+             })
+    )
+    else None
+
+let as_ms_hash_value h = lseq_u8_to_bv h
+let as_u8_hash_value h = bv_to_lseq_u8 h
+
+let hash_entry (e: ms_hashfn_dom)
+  : HA.hash_value_t
+  = match as_stamped_record e with
+    | None ->
+      unspecified_hash_function e
+    | Some r ->
+      let b = serializer r in
+      HA.hash_value b
+
+(*
+ * incremental multiset hash function - update the
+ * hash given a new element
+ *)
+let ms_hashfn_upd (e: ms_hashfn_dom) (h: ms_hash_value)
+  : Tot ms_hash_value
+  = as_ms_hash_value (
+        HA.aggregate_hash_value (as_u8_hash_value h)
+                                (hash_entry e)
+    )
+
+let lemma_mshashfn_correct (s1 s2: seq ms_hashfn_dom)
+  : Lemma (requires (seq2mset #_ #ms_hashfn_dom_cmp s1 ==
+                     seq2mset #_ #ms_hashfn_dom_cmp s2))
+          (ensures (ms_hashfn s1 = ms_hashfn s2))
+  = introduce forall x. Seq.count x s1 == Seq.count x s2
+    with (seq2mset_mem #_ #ms_hashfn_dom_cmp s1 x;
+          seq2mset_mem #_ #ms_hashfn_dom_cmp s2 x);
+    length_size #_ #ms_hashfn_dom_cmp s1;
+    length_size #_ #ms_hashfn_dom_cmp s2;
+    assert (Seq.length s1 == Seq.length s2);
+    admit()
+
+(* aggregation of multiset hashes *)
+let ms_hashfn_agg (h1: ms_hash_value) (h2: ms_hash_value)
+  : Tot ms_hash_value
+  = as_ms_hash_value (
+       HA.aggregate_hash_value
+         (as_u8_hash_value h1)
+         (as_u8_hash_value h2)
+    )
+
+// let ms_hashfn_agg_empty (h:ms_hash_value)
+//   : Lemma (ensures ms_hashfn_agg empty_hash_value h == h)
+//           [SMTPat (ms_hashfn_agg empty_hash_value h)]
+//   = admit()
+
+// let ms_hashfn_agg_sym (h0 h1:ms_hash_value)
+//   : Lemma (ensures ms_hashfn_agg h0 h1 ==
+//                    ms_hashfn_agg h1 h0)
+//            [SMTPat (ms_hashfn_agg h0 h1)]
+//   = admit()
+
+// let ms_hashfn_agg_assoc (h0 h1 h2:ms_hash_value)
+//   : Lemma (ensures ms_hashfn_agg h0 (ms_hashfn_agg h1 h2) ==
+//                    ms_hashfn_agg (ms_hashfn_agg h0 h1) h2)
+//            [SMTPat (ms_hashfn_agg h0 (ms_hashfn_agg h1 h2))]
+//   = admit()
+
+let agg_empty (h:u8_hash_value)
+  : Lemma (ensures HA.aggregate_hash_value (as_u8_hash_value empty_hash_value) h == h)
+          [SMTPat (HA.aggregate_hash_value (as_u8_hash_value empty_hash_value) h)]
+  = admit()
+
+let agg_sym (h0 h1:u8_hash_value)
+  : Lemma (ensures HA.aggregate_hash_value h0 h1 ==
+                   HA.aggregate_hash_value h1 h0)
+           [SMTPat (HA.aggregate_hash_value h0 h1)]
+  = admit()
+
+let agg_assoc (h0 h1 h2:u8_hash_value)
+  : Lemma (ensures HA.aggregate_hash_value h0 (HA.aggregate_hash_value h1 h2) ==
+                   HA.aggregate_hash_value (HA.aggregate_hash_value h0 h1) h2)
+           [SMTPat (HA.aggregate_hash_value h0 (HA.aggregate_hash_value h1 h2))]
+  = admit()
+
+let inverse_hash_value_conversion1 (h:ms_hash_value)
+  : Lemma (as_ms_hash_value (as_u8_hash_value h) == h)
+          [SMTPat (as_ms_hash_value (as_u8_hash_value h))]
+  = admit()
+let inverse_hash_value_conversion2 (h:u8_hash_value)
+  : Lemma (as_u8_hash_value (as_ms_hash_value h) == h)
+          [SMTPat (as_u8_hash_value (as_ms_hash_value h))]
+  = admit()
+
+
+let rec lemma_hashfn_agg (s1 s2: seq ms_hashfn_dom)
+  : Lemma
+    (ensures ms_hashfn (append s1 s2) = ms_hashfn_agg (ms_hashfn s1) (ms_hashfn s2))
+    (decreases (Seq.length s2))
+  = reveal_opaque (`%ms_hashfn) ms_hashfn;
+    if Seq.length s2 = 0
+    then (
+      assert (Seq.append s1 s2 `Seq.equal` s1);
+      assert (ms_hashfn s2 == empty_hash_value)
+    )
+    else (
+      let n = Seq.length s2 - 1 in
+      let s2' = SeqAux.prefix s2 n in
+      let last = Seq.index s2 n in
+      lemma_hashfn_agg s1 s2';
+      assert (Seq.equal (append s1 s2)
+                        (Seq.snoc (append s1 s2') last));
+      assert (Seq.equal (SeqAux.prefix (append s1 s2) (Seq.length (append s1 s2) - 1))
+                        (append s1 s2'));
+      assert (ms_hashfn (append s1 s2) ==
+              ms_hashfn_agg (ms_hashfn (append s1 s2'))
+                            (as_ms_hash_value (hash_entry last))))
+
+let ms_hashfn_sym (s1 s2: seq ms_hashfn_dom)
+  : Lemma
+    (ensures ms_hashfn (append s1 s2) = ms_hashfn (append s2 s1))
+  = lemma_hashfn_agg s1 s2;
+    lemma_hashfn_agg s2 s1
